\section*{Exercise 1}
Let $R=(r_{i}^{(s)})$ a payoff matrix with $R^{(t)}=\sum_{i=1}^{n}p_{i}^{(t)}r_{i}^{(s)}$

We see that the weight update rule depends on the payoff matrix :
\[\omega_{i}^{(t+1)}=\omega_{i}^{(t)}(1+\alpha R_{it})\]

We have the potential function: 
\[\Phi^{(t)}=\sum_{i=1}^{n}\omega _{i}^{(t)}\]

So : 
\[\Phi^{(t+1)}=\sum_{i=1}^{n}\omega _{i}^{(t)}(1+\alpha R_{it})\]
\[\Phi^{(t+1)}=\sum_{i=1}^{n}\omega _{i}^{(t)}+\sum_{i=1}^{n}\omega _{i}^{(t)}\alpha R_{it}\]
\[\Phi^{(t+1)}\leqslant \Phi^{(t)}+\alpha \sum_{i=1}^{n}\omega _{i}^{(t)}\]
\[\Phi^{(t+1)}\leqslant (1+\alpha )\Phi^{(t)}\]

By induction we can find:
\[\Phi^{(t+1)}\leqslant n(1+\alpha )^{t} \left ( * \right )\]


So:
\[\sum_{i=1}^{n}\omega _{i}^{(t+1)}\leqslant n(1+\alpha )^{t}\]

\[\omega _{i}^{(t+1)}\leqslant n(1+\alpha )^{t}\]

\[\prod_{s=1}^{t}(1+\alpha R_{it})\leqslant n(1+\alpha )^{t}\]
\[ln(\prod_{s=1}^{t}(1+\alpha R_{it}))\leqslant ln(n(1+\alpha )^{t})\]
\[\sum_{s=1}^{t}ln((1+\alpha R_{it}))\leqslant ln(n)+ t*ln(1+\alpha )\]
\[\frac{\sum_{s=1}^{t}ln((1+\alpha R_{it}))-ln(n)}{ln(1+\alpha)} \leqslant t\]

From the inequality (3) given in the hint we find: 

\[\frac{1}{ln(1+\alpha )}\geqslant \frac{1}{\alpha }\]

From the inequality (2) given in the hint we find: 
 
\[ln((1+\alpha R_{it}))\geqslant \alpha R_{it}(1-\alpha R_{it})\]
\[ln((1+\alpha R_{it}))\geqslant \alpha R_{it}(1-\alpha )\]

So finally we find :
\[\frac{\sum_{s=1}^{t}\alpha R_{it}(1-\alpha )-ln(n)}{\alpha} \leqslant t\]

It's easy to see that : 
\[t\leqslant \sum_{s=1}^{t}R^{(t)}\]

Thus:

\[\sum_{s=1}^{t} R_{it}(1-\alpha)+\frac{-ln(n)}{\alpha}  \leqslant \sum_{s=1}^{t}R^{(t)}\]